adding a concrete list of indices for non-zero sub-buffers

examples/low-mitls-experiments/HSL.fst
@@ -29,12 +29,14 @@ type loc = LowStar.Modifies.loc
  * So, the record layer appends to the buffer after p1
  * At some point (in HSL.process), HSL decides that the contents between p0 and p1 is a valid message
  * And at that point, it moves p0 and p1
+ * msgs is the list of all subsequences in the buffer that don't contain a 0ul
  *)
 abstract noeq type hsl_state =
   | Mk_state: len:u32 ->
-              buf: Buffer.buffer u32{Buffer.len buf == len} ->
+              buf:Buffer.buffer u32{Buffer.len buf == len} ->
               p0:reference u32 ->
 	      p1:reference u32 ->
+	      msgs:reference (list (u32 * u32)) ->
 	      hsl_state
 
 (* abstract getters *)
@@ -42,6 +44,7 @@ abstract let hsl_get_len (st:hsl_state) :u32 = st.len
 abstract let hsl_get_buf (st:hsl_state) :Buffer.buffer u32 = st.buf
 abstract let hsl_get_p0 (st:hsl_state) :reference u32 = st.p0
 abstract let hsl_get_p1 (st:hsl_state) :reference u32 = st.p1
+abstract let hsl_get_msgs (st:hsl_state) :reference (list (u32 * u32)) = st.msgs
 
 [@"opaque_to_smt"]
 unfold private let loc_pairwise_disjoint (s:TSet.set loc) :Type0 =
@@ -50,14 +53,15 @@ unfold private let loc_pairwise_disjoint (s:TSet.set loc) :Type0 =
 (* liveness and disjointness *)
 [@"opaque_to_smt"]
 unfold private let liveness_and_disjointness (st:hsl_state) (h:mem) :Type0 =
-  let len, buf, p0, p1 = hsl_get_len st, hsl_get_buf st, hsl_get_p0 st, hsl_get_p1 st in
+  let len, buf, p0, p1, msgs = hsl_get_len st, hsl_get_buf st, hsl_get_p0 st, hsl_get_p1 st, hsl_get_msgs st in
   
   //we used to have !{} syntax, which is now repurposed for Set, would be nice to have some such syntax for TSet
   loc_pairwise_disjoint (TSet.union (TSet.singleton (Mods.loc_mreference p0))
                                     (TSet.union (TSet.singleton (Mods.loc_mreference p1))
-				                (TSet.singleton (Mods.loc_buffer buf)))) /\  //disjointness
+				                (TSet.union (TSet.singleton (Mods.loc_buffer buf))
+						            (TSet.singleton (Mods.loc_mreference msgs))))) /\
 
-  Buffer.live h buf /\ contains h p0 /\ contains h p1 /\  //liveness
+  Buffer.live h buf /\ contains h p0 /\ contains h p1 /\ contains h msgs /\  //liveness
   Buffer.len buf == len /\  //buffer length
   sel h p0 <=^ len /\  //p0 and p1 invariants
   sel h p1 <=^ len /\
@@ -72,16 +76,33 @@ unfold private let null_terminator_invariant_buf
     let subseq = Buffer.as_seq h (Buffer.gsub buf p0 subseq_size) in
     forall (i:nat). i < v subseq_size ==> Seq.index subseq i =!= 0ul
 
+[@"opaque_to_smt"]
+unfold private let msgs_list_invariant_buf
+  (len:u32) (buf:Buffer.buffer u32) (l:list (u32 * u32)) (p0:u32{p0 <=^ len})
+  (h:mem{Buffer.len buf == len}) :GTot Type0
+  = forall (i j:u32). List.Tot.mem (i, j) l ==>
+                 (i <^ j /\ j <^ p0 /\
+		  (let subseq_size = j -^ i in
+		   let subseq = Buffer.as_seq h (Buffer.gsub buf i subseq_size) in
+		   forall (k:nat). k < v subseq_size ==> Seq.index subseq k =!= 0ul))
+
 (* an invariant on the sequence content between p0 and p1 in the buffer *)
 [@"opaque_to_smt"]
 unfold private let null_terminator_invariant (st:hsl_state) (h:mem{liveness_and_disjointness st h}) :GTot Type0 
   = let buf, p0, p1 = hsl_get_buf st, sel h (hsl_get_p0 st), sel h (hsl_get_p1 st) in
     null_terminator_invariant_buf (hsl_get_len st) buf p0 p1 h
 
+(* an invariant on the list of indices *)
+[@"opaque_to_smt"]
+unfold private let msgs_list_invariant (st:hsl_state) (h:mem{liveness_and_disjointness st h}) :GTot Type0 
+  = let len, buf, p0, msgs = hsl_get_len st, hsl_get_buf st, sel h (hsl_get_p0 st), sel h (hsl_get_msgs st) in
+    msgs_list_invariant_buf len buf msgs p0 h
+
 [@"opaque_to_smt"]
 unfold private let hsl_invariant_predicate (st:hsl_state) (h:mem) :Type0 =
   liveness_and_disjointness st h /\
-  null_terminator_invariant st h
+  null_terminator_invariant st h /\
+  msgs_list_invariant st h
 
 (* finally, the abstract invariant and its elimination *)
 abstract let hsl_invariant (st:hsl_state) (h:mem) :Type0 = hsl_invariant_predicate st h
@@ -99,11 +120,13 @@ let lemma_hsl_invariant_elim (st:hsl_state) (h:mem)
 let hsl_footprint (st:hsl_state) (h:mem{hsl_invariant st h}) =
   loc_union (loc_union (loc_buffer (Buffer.gsub (hsl_get_buf st) 0ul (sel h (hsl_get_p1 st))))
 		       (loc_mreference (hsl_get_p0 st)))
-	    (loc_mreference (hsl_get_p1 st))
+	    (loc_union (loc_mreference (hsl_get_p1 st))
+	               (loc_mreference (hsl_get_msgs st)))
 
 (*
  * Framing the HSL invariant across its footprint
  *)
+#set-options "--z3rlimit 30"
 let lemma_frame_hsl_invariant (st:hsl_state) (l:loc) (h0 h1:mem)
   :Lemma (requires (hsl_invariant st h0                  /\
                     loc_disjoint l (hsl_footprint st h0) /\
@@ -111,21 +134,30 @@ let lemma_frame_hsl_invariant (st:hsl_state) (l:loc) (h0 h1:mem)
 	 (ensures  (hsl_invariant st h1 /\ hsl_footprint st h1 == hsl_footprint st h0))
 	 [SMTPat (hsl_invariant st h0); SMTPat (loc_disjoint l (hsl_footprint st h0));
 	  SMTPat (Mods.modifies l h0 h1)]
-  = let buf, p0, p1 = hsl_get_buf st, hsl_get_p0 st, hsl_get_p1 st in
+  = let buf, p0', p1, msgs = hsl_get_buf st, hsl_get_p0 st, hsl_get_p1 st, hsl_get_msgs st in
 
     let b0 = Buffer.as_seq h0 buf in
+    let b1 = Buffer.as_seq h0 buf in
+    let p0 = v (sel h0 p0') in
     let p1 = v (sel h0 p1) in
+
+    let msgs0 = sel h0 msgs in
+    let msgs1 = sel h1 msgs in
+    assert (msgs0 == msgs1);
 
     //we need this to prove the uncommented part below, essentially that the buffer
     //contents did not change between p0 and p1
     //we have buffer contents did not change from 0 to p1,
     //it is a bit unfortunate that from that we can't SMT derive between p0 to p1
-    assert (forall (k:nat). k < p1 ==> Seq.index b0 k == Seq.index (Seq.slice b0 0 p1) k)
+    assert (forall (k:nat). k < p1 ==> Seq.index b0 k == Seq.index (Seq.slice b0 0 p1) k);
+    assert (forall (i j:nat) (k:nat). (i < j /\ j < p0 /\ k < (j - i)) ==>
+                              Seq.index (Seq.slice b0 i j) k == Seq.index (Seq.slice b1 i j) k)
     // assert (Seq.equal (Buffer.as_seq h0 (Buffer.gsub buf (sel h0 p0) (sel h0 p1 -^ sel h0 p0)))
     //                   (Buffer.as_seq h1 (Buffer.gsub buf (sel h1 p0) (sel h1 p1 -^ sel h1 p0))))
 
 assume val fresh_loc: Mods.loc -> mem -> mem -> Type0
 
+#reset-options
 (*
  * Creating of HSL state
  * Assuming freshness and disjointness for now
@@ -137,36 +169,46 @@ let hsl_create (len:u32{len >^ 0ul})
 		                        fresh_loc (loc_buffer (hsl_get_buf st)) h0 h1    /\
 					fresh_loc (loc_mreference (hsl_get_p0 st)) h0 h1 /\
 					fresh_loc (loc_mreference (hsl_get_p1 st)) h0 h1 /\
+					fresh_loc (loc_mreference (hsl_get_msgs st)) h0 h1 /\
 		                        Mods.modifies loc_none h0 h1))
   = let h0 = ST.get () in
     let buf = Buffer.gcmalloc root 0ul len in
     let p0 = ralloc root 0ul in
     let p1 = ralloc root 0ul in
+    let msgs = ralloc root [] in
     let h2 = ST.get () in
-    let st = Mk_state len buf p0 p1 in
+    let st = Mk_state len buf p0 p1 msgs in
     assume (fresh_loc (loc_buffer (hsl_get_buf st)) h0 h2);
     assume (fresh_loc (loc_mreference (hsl_get_p0 st)) h0 h2);
     assume (fresh_loc (loc_mreference (hsl_get_p1 st)) h0 h2);
+    assume (fresh_loc (loc_mreference (hsl_get_msgs st)) h0 h2);
     assume (loc_pairwise_disjoint (TSet.union (TSet.singleton (Mods.loc_mreference p0))
                                               (TSet.union (TSet.singleton (Mods.loc_mreference p1))
-				                          (TSet.singleton (Mods.loc_buffer buf)))));
+				                          (TSet.union (TSet.singleton (Mods.loc_buffer buf))
+							              (TSet.singleton (Mods.loc_mreference msgs))))));
     st
 
 (*
  * Auxiliary function for processing the buffer, skip ahead
  *)
-private let rec aux_process (len:u32) (b:Buffer.buffer u32) (p0 p1 p:u32)
-  :ST u32 (requires (fun h0      -> Buffer.live h0 b /\
-                                 len == Buffer.len b /\ p <=^ len /\ p1 <=^ p /\ p0 <=^ p1 /\
-                                 null_terminator_invariant_buf len b p0 p1 h0))
-          (ensures  (fun h0 r h1 -> Buffer.live h1 b /\ 
-	                         r <=^ p /\ null_terminator_invariant_buf len b r p h1 /\
-	                         Mods.modifies loc_none h0 h1))
-  = if p = p1 then p0
+private let rec aux_process (len:u32) (b:Buffer.buffer u32) (p0 p1 p:u32) (l:list (u32 * u32))
+  :ST (u32 * list (u32 * u32))
+      (requires (fun h0 -> Buffer.live h0 b /\
+                        len == Buffer.len b /\ p <=^ len /\ p1 <=^ p /\ p0 <=^ p1 /\
+                        null_terminator_invariant_buf len b p0 p1 h0 /\
+			msgs_list_invariant_buf len b l p0 h0))
+      (ensures  (fun h0 (r, l) h1 -> Buffer.live h1 b /\ 
+	                          r <=^ p /\
+				  null_terminator_invariant_buf len b r p h1 /\
+				  msgs_list_invariant_buf len b l r h1 /\
+	                          Mods.modifies loc_none h0 h1))
+  = if p = p1 then p0, l
     else
       let c = Buffer.index b p1 in
-      if c = 0ul then aux_process len b (p1 +^ 1ul) (p1 +^ 1ul) p
-      else aux_process len b p0 (p1 +^ 1ul) p
+      if c = 0ul then
+        if p0 = p1 then aux_process len b (p1 +^ 1ul) (p1 +^ 1ul) p l
+        else aux_process len b (p1 +^ 1ul) (p1 +^ 1ul) p ((p0, p1)::l)
+      else aux_process len b p0 (p1 +^ 1ul) p l
 
 (*
  * Main process function that client (Record) calls once it has appended some data to the input buffer
@@ -181,7 +223,8 @@ let hsl_process (st:hsl_state) (p:u32)
 	                          sel h1 (hsl_get_p1 st) == p /\  //p1 has been updated to p
 	                          Mods.modifies (Mods.loc_union (Mods.loc_mreference (hsl_get_p0 st))
 				                                (Mods.loc_mreference (hsl_get_p1 st))) h0 h1))
-  = let len, buf, p0, p1 = hsl_get_len st, hsl_get_buf st, hsl_get_p0 st, hsl_get_p1 st in
-    let new_p0 = aux_process len buf (!p0) (!p1) p in
+  = let len, buf, p0, p1, msgs = hsl_get_len st, hsl_get_buf st, hsl_get_p0 st, hsl_get_p1 st, hsl_get_msgs st in
+    let new_p0, new_msgs = aux_process len buf (!p0) (!p1) p (!msgs) in
     p0 := new_p0;
-    p1 := p
+    p1 := p;
+    msgs := new_msgs
